lakefile.lean
@@ -43,9 +43,9 @@ target vampire_ffi.o pkg : FilePath := do
   let flags := vampireCompileArgs ++ #["-I", (← getLeanIncludeDir).toString, "-fPIC"]
   buildO oFile srcJob flags #[] "c++"
 
-target vampire_problem.o pkg : FilePath := do
-  let oFile := pkg.buildDir / "ffi" / "vampire_problem.o"
-  let srcJob ← inputTextFile <| pkg.dir / "ffi" / "vampire_problem.cpp"
+target vampire_proof.o pkg : FilePath := do
+  let oFile := pkg.buildDir / "ffi" / "vampire_proof.o"
+  let srcJob ← inputTextFile <| pkg.dir / "ffi" / "vampire_proof.cpp"
   let flags := vampireCompileArgs ++ #["-I", (← getLeanIncludeDir).toString, "-fPIC"]
   buildO oFile srcJob flags #[] "c++"
 
@@ -70,7 +70,7 @@ target vampire_archive : FilePath := do
 extern_lib libvampireffi pkg := do
   let name := nameToStaticLib "vampireffi"
   let ffiO ← fetch <| pkg.target ``vampire_ffi.o
-  let probO ← fetch <| pkg.target ``vampire_problem.o
   let buildO ← fetch <| pkg.target ``vampire_build.o
+  let proofO ← fetch <| pkg.target ``vampire_proof.o
   let _ ← fetch <| pkg.target ``vampire_archive
-  buildStaticLib (pkg.staticLibDir / name) #[ffiO, probO, buildO]
+  buildStaticLib (pkg.staticLibDir / name) #[ffiO, buildO, proofO]
